src-lite/bidirectional.v
@@ -8,45 +8,6 @@ Require Import bidir.elaboration.
 Require Import ln_utils.
 
 
-(* Theorem bidir_complete1 : forall Γ e1 e2 A
-  , Γ ⊢ e1 <: e2 : A
-  → to_bcontext Γ ⊢ to_bexpr e1 <: to_bexpr e2 ⇒ to_bexpr A.
-Proof.
-  induction 1.
-
-  1-9: admit.
-  - simpl. econstructor.
-    eapply bs_castup with (B := (to_bexpr B)).
-    + admit.
-    + admit.
-(*
-  1-14: admit.
-  - admit. *)
-Admitted. *)
-
-(* Theorem bidir_complete2 : forall Γ e1 e2 A
-  , Γ ⊢ e1 <: e2 : A
-  → to_bcontext Γ ⊢ to_bexpr e1 <: to_bexpr e2 ⇐ to_bexpr A.
-Proof.
-  induction 1.
-  1-7: admit.
-  - admit.
-Admitted. *)
-
-(* dummy condition *)
-(* Definition ctx_condition : context → bcontext → Prop := fun c c' => True.
-Definition condition : expr → bexpr → Prop := fun e e' => True.
-
-Theorem bidir_complete3 : forall Γ e1 e2 A
-  , Γ ⊢ e1 <: e2 : A
-  → exists Γ' e1' e2' A', Γ' ⊢ e1' <: e2' ⇒ A' ∧ ctx_condition Γ Γ'
-    ∧ condition e1 e1' ∧ condition e2 e2' ∧ condition A A'.
-Proof.
-  induction 1.
-  1-6: admit.
-  - admit.
-Admitted. *)
-
 Ltac destruct_mono :=
   repeat
     match goal with
@@ -63,18 +24,20 @@ Lemma usub_elab_keeps_mono : forall Γ e1 e2 A Γ' e1' e2' A',
    usub_elab Γ e1 e2 A Γ' e1' e2' A' ->
        (mono_type e1 /\ mono_type e2 -> mono_btype e1' /\ mono_btype e2') /\ lc_bexpr e1' /\ lc_bexpr e2'.
 Proof.
- intros.
- induction H; repeat split; destruct_conjs; intros; auto; try solve_trivial_mono; try solve_lc_bexpr.
- - destruct_mono. econstructor. solve_lc_bexpr. 
-  + eapply bmono_lambda with (L:=L `union` (L0 `union` L1)). intros. inst_cofinites_with x. intuition. 
- - destruct_mono. econstructor. solve_lc_bexpr.
-  + eapply bmono_lambda with (L:=L `union` (L0 `union` L1)). intros. inst_cofinites_with x. intuition. 
- - destruct_mono. eapply bmono_pi with (L:=L `union` (L0 `union` L1)). intuition. intros. inst_cofinites_with x. intuition.
- - destruct_mono. eapply bmono_pi with (L:=L `union` (L0 `union` L1)). intuition. intros. inst_cofinites_with x. intuition.
- - destruct_mono. econstructor. solve_lc_bexpr.
-   eapply bmono_bind with (L:=L `union` (L0 `union` L1)). intros. inst_cofinites_with x. intuition.
- - destruct_mono. econstructor. solve_lc_bexpr.
-   eapply bmono_bind with (L:=L `union` (L0 `union` L1)). intros. inst_cofinites_with x. intuition.
+  intros.
+  induction H; repeat split; destruct_conjs; intros; auto; try solve_trivial_mono; try solve_lc_bexpr.
+  - destruct_mono. eapply bmono_lambda with (L:=L `union` (L0 `union` L1)). intuition. solve_lc_bexpr. 
+    intros. inst_cofinites_with x. intuition. 
+  - destruct_mono. eapply bmono_lambda with (L:=L `union` (L0 `union` L1)). intuition. solve_lc_bexpr. 
+    intros. inst_cofinites_with x. intuition. 
+  - destruct_mono. eapply bmono_pi with (L:=L `union` (L0 `union` L1)). intuition. 
+    intros. inst_cofinites_with x. intuition.
+  - destruct_mono. eapply bmono_pi with (L:=L `union` (L0 `union` L1)). intuition. 
+    intros. inst_cofinites_with x. intuition.
+  - destruct_mono. eapply bmono_bind with (L:=L `union` (L0 `union` L1)). intuition. solve_lc_bexpr.
+    intros. inst_cofinites_with x. intuition.
+  - destruct_mono. eapply bmono_bind with (L:=L `union` (L0 `union` L1)). intuition. solve_lc_bexpr.
+    intros. inst_cofinites_with x. intuition.
 Qed.
 
 Scheme expr_ind_mut 
@@ -116,13 +79,31 @@ Lemma open_bexpr_wrt_new_var_keeps_notin_berase : forall x x' e n0,
   x <> x' -> x `notin` ott.fv_eexpr (berase e) <-> x `notin` ott.fv_eexpr (berase (open_bexpr_wrt_bexpr_rec n0 `'x' e)).
 Proof.
   intros; split; intros.
-  - generalize dependent n0. generalize dependent H0.
-    induction e; intros; auto; try (simpl in *; auto; fail).
+  - generalize dependent n0. generalize dependent H0. pattern e.
+    eapply bexpr_mut with 
+    (P0 := fun b => 
+      match b with 
+      | bb_anno e A => forall n0, 
+          x `notin` ott.fv_eexpr (berase e) ->
+          x `notin` ott.fv_eexpr (berase (open_bexpr_wrt_bexpr_rec n0 `'x' e))
+      end
+    ); intros; auto; try (simpl in *; auto; fail).
     + simpl. destruct (lt_eq_lt_dec n n0); simpl.
       * destruct s; simpl; auto.
       * auto.
-  - generalize dependent n0. 
-    induction e; intros; auto; try (simpl in *; eauto).
+    + destruct b; simpl in *; auto. 
+    + destruct b; simpl in *; auto.
+  - generalize dependent n0. pattern e.
+    eapply bexpr_mut with 
+    (P0 := fun b => 
+      match b with 
+      | bb_anno e A => forall n0, 
+          x `notin` ott.fv_eexpr (berase (open_bexpr_wrt_bexpr_rec n0 `'x' e)) ->
+          x `notin` ott.fv_eexpr (berase e)
+      end
+    ); intros; auto; try (simpl in *; eauto; fail).  
+    + destruct b; simpl in *. eauto. 
+    + destruct b; simpl in *. eauto.
 Qed.
 
 Ltac convert_to_open_expr_wrt_new_var := 
@@ -130,8 +111,8 @@ Ltac convert_to_open_expr_wrt_new_var :=
   | H : ?x `notin` ott.fv_eexpr (erase ?e) |- ?x `notin` ott.fv_eexpr (berase ?e') =>  
       match goal with 
       | H1 : ?x `notin` ott.fv_eexpr (erase (?e ^^ `?x0)) -> ?x `notin` ott.fv_eexpr (berase (?e' ^^' `' ?x0)) |- _ => 
-        eapply open_expr_wrt_new_var_keeps_notin_erase with (x':=x0) (n0:=0) in H; eauto;
-        specialize (H1 H); eapply open_bexpr_wrt_new_var_keeps_notin_berase with (n0:=0); eauto                                     
+        eapply open_expr_wrt_new_var_keeps_notin_erase with (x':=x0) (n0:=0) in H; eauto 3;
+        specialize (H1 H); eapply open_bexpr_wrt_new_var_keeps_notin_berase with (n0:=0); eauto 3                             
       end 
   end.
 
@@ -149,6 +130,44 @@ Proof.
     convert_to_open_expr_wrt_new_var. 
   - apply notin_union; auto. apply notin_union_2 in H0.
     convert_to_open_expr_wrt_new_var.
+Qed.
+
+Lemma usub_elab_keeps_notin_fv_erase_helper : forall x x' e e',
+  x <> x' ->
+  x `notin` ott.fv_eexpr (erase e) -> 
+  (x `notin` ott.fv_eexpr (erase (e ^^ ` x')) -> x `notin` ott.fv_eexpr (berase (e' ^^' `' x'))) ->
+  x `notin` ott.fv_eexpr (berase e').
+Proof.
+  intros.
+  convert_to_open_expr_wrt_new_var.
+Qed.
+
+Lemma usub_elab_keeps_notin_fv_erase : forall Γ e1 e2 A Γ' e1' e2' A' x,
+   usub_elab Γ e1 e2 A Γ' e1' e2' A' -> 
+      (x `notin` ott.fv_eexpr (erase e1) ->  x `notin` ott.fv_eexpr (berase e1')) /\
+      (x `notin` ott.fv_eexpr (erase e2) ->  x `notin` ott.fv_eexpr (berase e2')).
+Proof.
+  intros.
+  induction H; try (simpl in *; auto; fail); simpl in *; inst_cofinites_by (add x L); destruct_conjs; split; intros.
+  - eapply usub_elab_keeps_notin_fv_erase_helper with (e:=e1) (x':=x0); eauto.
+  - eapply usub_elab_keeps_notin_fv_erase_helper with (e:=e2) (x':=x0); eauto.
+  - apply notin_union.
+    + auto.
+    + eapply usub_elab_keeps_notin_fv_erase_helper with (e:=B1) (x':=x0); eauto.
+  - apply notin_union. auto.
+    eapply usub_elab_keeps_notin_fv_erase_helper with (e:=B2) (x':=x0); eauto.
+  - eapply usub_elab_keeps_notin_fv_erase_helper with (e:=e1) (x':=x0); eauto.
+  - eapply usub_elab_keeps_notin_fv_erase_helper with (e:=e2) (x':=x0); eauto.
+  - apply notin_union. auto. apply notin_union_2 in H12.
+    eapply usub_elab_keeps_notin_fv_erase_helper with (e:=B) (x':=x0); eauto.
+  - auto.
+  - auto.
+  - apply notin_union. auto.
+    eapply usub_elab_keeps_notin_fv_erase_helper with (e:=C) (x':=x0); eauto.
+  - apply notin_union. auto.
+    eapply usub_elab_keeps_notin_fv_erase_helper with (e:=B) (x':=x0); eauto.
+  - apply notin_union. auto.
+    eapply usub_elab_keeps_notin_fv_erase_helper with (e:=C) (x':=x0); eauto.
 Qed.
 
 Ltac convert_match_to_open_bexpr_wrt_new_var := 
@@ -193,19 +212,6 @@ Ltac destruct_notin_union :=
     | H : ?x `notin` ?s `union` ?s' |- _ => apply notin_union_equiv_notin_conj in H; destruct_conjs
     end.
 
-
-Lemma busub_elab_keeps_notin_fv_erase : forall Γ' e1' e2' d' A' Γ e1 e2 A x,
-   busub_elab Γ' e1' e2' d' A' Γ e1 e2 A -> 
-   (x `notin` ott.fv_eexpr (berase e1') -> x `notin` ott.fv_eexpr (erase e1)) /\
-   (x `notin` ott.fv_eexpr (berase e2') -> x `notin` ott.fv_eexpr (erase e2)).
-Proof.
-  intros.
-  induction H; try (simpl in *; split; destruct_conjs; auto); inst_cofinites_by (add x L); intros; destruct_conjs;
-    try (convert_match_to_open_bexpr_wrt_new_var; eauto);
-    try (destruct_notin_union; apply notin_union; auto; convert_match_to_open_bexpr_wrt_new_var; eauto).
-Qed.
-    
-
 Lemma wf_context_elab_same_dom : forall Γ Γ',
     wf_context_elab Γ Γ' -> ctx_dom Γ = bctx_dom Γ'.
 Proof.
@@ -223,34 +229,20 @@ Proof with eauto with bidir.
     (P0 := 
       fun Γ Γ' (_ : wf_context_elab Γ Γ') => wf_bcontext Γ'); 
     intros; try (constructor; auto; fail).
-  - econstructor; auto; eauto...
-  - econstructor; intros.
-    + econstructor; eauto...
-      * intros. inst_cofinites_with x. eapply bs_sub with (A:=B1' ^`' x)...
-    + eapply bs_pi with (L:=L); eauto...
-    + eapply bs_pi with (L:=L); eauto...
-  - econstructor; eauto... 
+  - eauto.
+  - eapply bs_abs; eauto...
+  - eauto...
   - econstructor; eauto...
     + eapply usub_elab_keeps_mono; eauto.
     + constructor; eapply busub_all_lc; eauto.
-  - eapply bs_anno.
-    + eapply bs_bind with (L:=L).
-      * eauto...
-      * intros. inst_cofinites_with x. eauto... 
-      * intros. eapply bs_sub.
-        inst_cofinites_with x. eauto...
-        eauto...
-      * intros. simpl. inst_cofinites_with x. eapply usub_elab_keeps_notin_fv_erase_l; eauto. 
-      * intros. simpl. inst_cofinites_with x. eapply usub_elab_keeps_notin_fv_erase_l; eauto.
-    + eauto... 
-    + eapply bs_forall with (L:=L); eauto...
-  - econstructor; eauto.
-    eapply bs_castup with (B:=B'); eauto.
-    + eapply bidir_refl_l in H0. exact H0.
-    + admit. (* breduce *)
-    + eapply bs_sub with (A:=B'). auto. admit. (* type_correctness *)
-  - admit.
-   (* eapply bs_castdn. exact H0. admit. breduce auto. *)
+  - eapply bs_bind with (L:=L) (A1:=A1'); eauto; intros;
+    inst_cofinites_with x; eauto...
+    eapply bs_sub; eauto. eapply bs_star_inf. eapply busub_context_is_wf; eauto.
+    eapply bs_sub; eauto. eapply bs_star_inf. eapply busub_context_is_wf; eauto.
+    eapply usub_elab_keeps_notin_fv_erase with (e1':=(e1'0 ^^' `' x)) (e2':=(e2'0 ^^' `' x)); eauto.
+    eapply usub_elab_keeps_notin_fv_erase with (e1':=(e1'0 ^^' `' x)) (e2':=(e2'0 ^^' `' x)); eauto.
+  - eapply bs_castup with (B:=B'); eauto. admit. admit. admit.
+  - eapply bs_anno; eauto... admit.
   - eapply bs_forall_l with (t:=t'); eauto...
     + eapply usub_elab_keeps_mono; eauto. 
   - econstructor; eauto.
@@ -272,51 +264,188 @@ Proof.
   - simpl. admit. 
 Admitted. *)
 
-Ltac destruct_bmono :=
-  repeat
-    match goal with
-    | H : mono_btype (?P ?x) |- _ => dependent destruction H
-    end.
+Theorem to_decl_open_expr_wrt_expr_distr_rec : forall e1 e2 n,
+  to_decl (open_bexpr_wrt_bexpr_rec n e2 e1) = open_expr_wrt_expr_rec n (to_decl e2) (to_decl e1).
+Proof.
+  intro e1. pattern e1.
+  eapply bexpr_mut with 
+  ( P0 := fun ( b : bbody ) => 
+    forall e2 n, to_body (open_bbody_wrt_bexpr_rec n e2 b) = open_body_wrt_expr_rec n (to_decl e2) (to_body b)); intros; auto;
+  try (simpl; rewrite <- H; auto; rewrite <- H0; auto; fail).
+  - simpl. destruct (lt_eq_lt_dec n n0); simpl; auto.
+    + destruct s; auto.
+Qed.
 
-Ltac solve_trivial_bmono := 
-    destruct_bmono; try solve [intuition | econstructor; intuition; eauto]; fail.   
-        
+Theorem to_decl_open_body_wrt_expr_distr_rec : forall b e n,
+  to_body (open_bbody_wrt_bexpr_rec n e b) = open_body_wrt_expr_rec n (to_decl e) (to_body b).
+Proof.
+  intro b. pattern b.
+  eapply bbody_mut with 
+    ( P := fun e1 => 
+      forall e2 n, to_decl (open_bexpr_wrt_bexpr_rec n e2 e1) = open_expr_wrt_expr_rec n (to_decl e2) (to_decl e1))
+    ( P0 := fun b => 
+      forall e n, to_body (open_bbody_wrt_bexpr_rec n e b) = open_body_wrt_expr_rec n (to_decl e) (to_body b)); 
+    intros; auto;
+  try (simpl; rewrite <- H; auto; rewrite <- H0; auto; fail).
+  - simpl. destruct (lt_eq_lt_dec n n0); simpl; auto.
+    + destruct s; auto.
+Qed.
 
-Lemma busub_elab_keeps_mono : forall Γ' e1' e2' d A' Γ e1 e2 A,
-   busub_elab Γ' e1' e2' d A' Γ e1 e2 A ->
-       (mono_btype e1' /\ mono_btype e2' -> mono_type e1 /\ mono_type e2) /\ lc_expr e1 /\ lc_expr e2.
+
+Theorem to_decl_open_expr_wrt_expr_distr : forall e1 e2,
+  to_decl (open_bexpr_wrt_bexpr e1 e2) = open_expr_wrt_expr (to_decl e1) (to_decl e2).
+Proof.
+  intros. unfold open_bexpr_wrt_bexpr. unfold open_expr_wrt_expr.
+  rewrite to_decl_open_expr_wrt_expr_distr_rec. auto.
+Qed.
+
+Theorem to_decl_open_body_wrt_expr_distr : forall b1 e2,
+  to_body (open_bbody_wrt_bexpr b1 e2) = open_body_wrt_expr (to_body b1) (to_decl e2).
+Proof. 
+  intros. unfold open_bbody_wrt_bexpr. unfold open_body_wrt_expr.
+  rewrite to_decl_open_body_wrt_expr_distr_rec. auto.
+Qed.
+
+
+Theorem to_decl_open_expr_wrt_var_distr : forall e1 x,
+  to_decl (e1 ^^' `'x)  = to_decl e1 ^^ `x.
 Proof.
   intros.
-  induction H; repeat split; destruct_conjs; intros; auto; try solve_trivial_bmono; try solve_lc_expr.
-  - destruct_bmono. eapply mono_lambda with (L:= L `union` L0 `union` L1); auto.
-    + solve_lc_expr.
-    + intros. inst_cofinites_with x; intuition.
-  - destruct_bmono. eapply mono_lambda with (L:= L `union` L0 `union` L1); auto.
-    + solve_lc_expr. 
-    + intros. inst_cofinites_with x; intuition.
-  - destruct_bmono. eapply mono_pi with (L:= L `union` L0 `union` L1).
-    + intuition.
-    + intros. inst_cofinites_with x. intuition.
-  - destruct_bmono. eapply mono_pi with (L:= L `union` L0 `union` L1).
-    + intuition.
-    + intros. inst_cofinites_with x. intuition.
-  - destruct_bmono. eapply mono_bind with (L:= L `union` L0 `union` L1); auto.
-    + solve_lc_expr. 
-    + intros. inst_cofinites_with x. intuition.
-  - destruct_bmono. eapply mono_bind with (L:= L `union` L0 `union` L1); auto.
-    + solve_lc_expr.
-    + intros. inst_cofinites_with x. intuition. 
+  replace (`x) with (to_decl `'x) by auto.
+  eapply to_decl_open_expr_wrt_expr_distr.
 Qed.
 
 
-Lemma wf_bcontext_elab_same_dom : forall Γ' Γ,
-  wf_bcontext_elab Γ' Γ -> bctx_dom Γ' = ctx_dom Γ.
+
+Ltac destruct_lc :=
+  match goal with 
+  | H : lc_bexpr (?P ?e1) |- _ => dependent destruction H
+  | H : lc_bexpr (?P ?e1 ?e2) |- _ => dependent destruction H
+  end.
+
+
+Theorem to_decl_keeps_lc : forall e,
+  lc_bexpr e -> lc_expr (to_decl e).
 Proof.
-  intros. induction H; auto.
-  simpl. rewrite IHwf_bcontext_elab; auto.
+  intros.
+  pattern e, H.
+  eapply lc_bexpr_mut with 
+    ( P0 := fun b (_ : lc_bbody b) =>
+        lc_body (to_body b)
+    ); intros; simpl; auto.
+  - constructor. auto. 
+    intros. replace (` x) with (to_decl (`' x)) by auto.
+    rewrite <- to_decl_open_body_wrt_expr_distr. auto.
+  - constructor; auto. intros.
+    rewrite <- to_decl_open_expr_wrt_var_distr. auto.
+  - econstructor; eauto. intros.
+    intros. replace (` x) with (to_decl (`' x)) by auto.
+    rewrite <- to_decl_open_body_wrt_expr_distr. auto.
+  - constructor; auto. intros.
+    rewrite <- to_decl_open_expr_wrt_var_distr. auto.
 Qed.
 
-Theorem bidir_sound : forall Γ' e1' e2' d A' Γ e1 e2 A,
+
+Theorem to_decl_keeps_mono : forall t, 
+  mono_btype t -> mono_type (to_decl t).
+Proof.
+  intros.
+  induction H; simpl; eauto.
+  - econstructor; now eapply to_decl_keeps_lc.
+  - eapply mono_pi with (L:=L); auto. intros. 
+    rewrite <- to_decl_open_expr_wrt_var_distr; auto.
+  - eapply mono_lambda with (L:=L); auto.
+    now eapply to_decl_keeps_lc.
+    replace  (λ_ to_decl A, to_decl e : to_decl B) with (to_decl ((λ, A, e : B))) by auto. now eapply to_decl_keeps_lc.
+    intros. replace (` x) with (to_decl (`' x)) by auto. rewrite <- to_decl_open_expr_wrt_expr_distr. auto.
+  - eapply mono_bind with (L:=L); auto. intros.
+    now eapply to_decl_keeps_lc.
+    replace  (Λ to_decl A, to_decl e : to_decl B) with (to_decl (Λ, A, e : B)) by auto. now eapply to_decl_keeps_lc.
+    intros. replace (` x) with (to_decl (`' x)) by auto. rewrite <- to_decl_open_expr_wrt_expr_distr. auto.
+  - eapply mono_castup; auto.
+    now eapply to_decl_keeps_lc.
+Qed.
+
+Hint Resolve to_decl_keeps_lc : lc.
+
+Theorem to_decl_keeps_reduce : forall A B,
+  breduce A B -> reduce (to_decl A) (to_decl B).
+Proof.
+  intros. induction H; simpl in *; eauto with lc. 
+  - rewrite to_decl_open_expr_wrt_expr_distr; econstructor; eauto with lc;
+    replace (λ_ to_decl A, to_decl e1 : to_decl B) with (to_decl ((λ, A, e1 : B))) by auto; now apply to_decl_keeps_lc.
+  - rewrite to_decl_open_expr_wrt_expr_distr. eapply r_inst;                 
+    try replace (Λ to_decl A, to_decl e1 : to_decl B) with (to_decl ((Λ, A, e1 : B))) by auto; try now apply to_decl_keeps_lc.
+    now apply to_decl_keeps_mono. 
+  - rewrite to_decl_open_expr_wrt_expr_distr. eapply r_cast_inst;
+    try replace (Λ to_decl A, to_decl e1 : to_decl B) with (to_decl ((Λ, A, e1 : B))) by auto; try now apply to_decl_keeps_lc.
+    now apply to_decl_keeps_mono.
+Qed.
+
+
+Theorem bidir_sound' : forall Γ e1 e2 d A,
+  busub Γ e1 e2 d A -> to_decl_context Γ ⊢ to_decl e1 <: to_decl e2 : to_decl A.
+Proof.
+  intros.
+  pattern Γ, e1, e2, d, A, H.
+  eapply busub_mut with 
+    ( P0 := fun Γ (_ : ⫦ Γ) => ⊢ to_decl_context Γ )
+    ( P1 := fun Γ A F (_ : infer_app Γ A F) => 
+      match F with 
+      | fun_pi B C => 
+        match A with 
+        | be_pi _ _ => True
+        | be_all _ _ => to_decl_context Γ ⊢ to_decl A : ⋆ -> 
+                        to_decl_context Γ ⊢ to_decl A <: e_pi (to_decl B) (to_decl C) : ⋆
+        | _ => False
+        end  
+      end
+    )
+    ( P2 := fun Γ A B (pf : Γ ⊢ A ⟼ B) =>
+      True ); 
+    intros; try (constructor; auto; fail).
+  - constructor; auto.
+    admit.
+  - simpl. eauto.
+  - simpl in *. eapply ott.s_abs with (L:=L); eauto;
+    intros; inst_cofinites_with x; repeat rewrite <- to_decl_open_expr_wrt_var_distr; eauto. 
+    + eapply narrowing_cons; eauto.
+    + eapply narrowing_cons; eauto.
+  - simpl in *. eapply ott.s_pi with (L:=L); eauto;
+    intros; inst_cofinites_with x; repeat rewrite <- to_decl_open_expr_wrt_var_distr; eauto.
+  - simpl in *. dependent destruction i.
+    + rewrite to_decl_open_expr_wrt_expr_distr. econstructor. 
+      now apply to_decl_keeps_mono. eauto.  replace (e_pi (to_decl B) (to_decl C)) with (to_decl (be_pi B C)) by auto.
+      auto.
+    + admit.
+  - simpl in *. eapply ott.s_bind with (L:=L); eauto; 
+    intros; repeat rewrite <- to_decl_open_expr_wrt_var_distr; eauto. 
+    + eapply narrowing_cons; eauto.
+    + eapply narrowing_cons; eauto.
+    + admit.
+    + admit.
+  - simpl in *. econstructor; eauto; eapply to_decl_keeps_reduce; eauto. 
+   - simpl in *. 
+    dependent destruction g.
+    + econstructor. eauto. eapply to_decl_keeps_reduce; eauto. eauto.
+    + admit. 
+    
+  - simpl in *. assert (mono_type (to_decl t)) by now apply to_decl_keeps_mono. eapply ott.s_forall_l with (L:=L); eauto.
+    + rewrite <- to_decl_open_expr_wrt_expr_distr. auto.
+    + intros. inst_cofinites_with x. rewrite <- to_decl_open_expr_wrt_var_distr. auto.
+  - simpl in *. eapply ott.s_forall_r with (L:=L); eauto.
+    intros. inst_cofinites_with x. rewrite <- to_decl_open_expr_wrt_var_distr. auto.
+  - simpl in *. eapply ott.s_forall with (L:=L); eauto.
+    intros. inst_cofinites_with x. repeat rewrite <- to_decl_open_expr_wrt_var_distr. auto.
+  - simpl in *; auto.
+  - eapply ott.s_sub with (A:=to_decl A0); eauto.
+
+  - admit.
+
+  - admit.
+Admitted.
+
+(* Theorem bidir_sound : forall Γ' e1' e2' d A' Γ e1 e2 A,
   busub_elab Γ' e1' e2' d A' Γ e1 e2 A → Γ ⊢ e1 <: e2 : A.
 Proof.
   intros.
@@ -394,4 +523,4 @@ Proof.
   (* P2 *)
   - admit. (* breduce *) 
   - admit. (* breduce *) 
-Admitted.
+Admitted. *)
